MathematicalLogic/FirstOrder/Theory.lean
@@ -3,25 +3,24 @@ import MathematicalLogic.FirstOrder.Bounded
 
 @[reducible] def Theory (𝓛) := Set (Sentence 𝓛)
 
-def Theory.toContext (𝓣 : Theory 𝓛) : Context 𝓛 :=
-  { BFormula.unbounded p | p ∈ 𝓣 }
+def Theory.ctx (𝓣 : Theory 𝓛) : Context 𝓛 :=
+  { BFormula.ub p | p ∈ 𝓣 }
 
-def Theory.Proof (𝓣 : Theory 𝓛) (p : Formula 𝓛) := 𝓣.toContext ⊢ p
+def Theory.Proof (𝓣 : Theory 𝓛) (p : Formula 𝓛) := 𝓣.ctx ⊢ p
 
-infix:50 " ⊢ " => Theory.Proof
+infix:50 " ⊢ᵀ " => Theory.Proof
 
 theorem Theory.axioms {p : Sentence 𝓛} {𝓣 : Theory 𝓛} :
-  p ∈ 𝓣 → 𝓣 ⊢ (p : Formula 𝓛) := by
+  p ∈ 𝓣 → 𝓣 ⊢ᵀ p.ub := by
   intro h
   apply Proof.assumption
   exists p
 
-lemma Theory.shift_eq {𝓣 : Theory 𝓛} : ↑ₚₛ𝓣.toContext = 𝓣.toContext := by
-  unfold Theory.toContext
-  simp [Context.lift, Sentence.shift_eq]
+lemma Theory.shift_eq {𝓣 : Theory 𝓛} : ↑ₚₛ𝓣.ctx = 𝓣.ctx := by
+  simp [ctx, Context.lift, Sentence.shift_eq]
 
 theorem Theory.generalization {𝓣 : Theory 𝓛} {p : Formula 𝓛} :
-  𝓣 ⊢ p → 𝓣 ⊢ ∀' p := by
+  𝓣 ⊢ᵀ p → 𝓣 ⊢ᵀ ∀' p := by
   intro h
   apply Proof.generalization
   rw [Theory.shift_eq]
@@ -44,12 +43,12 @@ instance : CoeOut (Model 𝓣) (Structure 𝓛) where
 end Model
 
 theorem Theory.soundness {𝓣 : Theory 𝓛} {p : Formula 𝓛} {𝓜 : Model 𝓣} {ρ : Assignment 𝓜} :
-  𝓣 ⊢ p → ⟦ p ⟧ₚ 𝓜, ρ := by
+  𝓣 ⊢ᵀ p → ⟦ p ⟧ₚ 𝓜, ρ := by
   intro h
   apply _root_.soundness
   · exact h
   · intro q ⟨p, h₁, h₂⟩
     subst h₂
-    simp [←Sentence.unbounded_interp_eq]
+    simp [←Sentence.ub_interp_eq]
     apply 𝓜.property
     exact h₁
