MathematicalLogic/Equality/Theory.lean
@@ -36,13 +36,17 @@ def BFormula.exists_unique (p : BFormula 𝓛 (m + 1)) :=
   ∃ᵇ (p ⋀ ∀ᵇ (↑ₚᵇp ⇒ #ᵇ1 ≈ᵇ #ᵇ0))
 prefix:max "∃ᵇ! " => BFormula.exists_unique
 
-@[simp] theorem Term.subst_eq {t₁ t₂ : Term 𝓛} : (t₁ ≈ t₂)[σ]ₚ = t₁[σ]ₜ ≈ t₂[σ]ₜ := by simp [Term.eq]
-@[simp] theorem Term.subst_neq {t₁ t₂ : Term 𝓛} : (t₁ ≉ t₂)[σ]ₚ = t₁[σ]ₜ ≉ t₂[σ]ₜ := by simp [Term.neq]
-@[simp] theorem Term.shift_eq {t₁ t₂ : Term 𝓛} : ↑ₚ(t₁ ≈ t₂) = ↑ₜt₁ ≈ ↑ₜ t₂ := Term.subst_eq
+@[simp] theorem Term.subst_eq {t₁ t₂ : Term 𝓛} :
+  (t₁ ≈ t₂)[σ]ₚ = t₁[σ]ₜ ≈ t₂[σ]ₜ := by simp [Term.eq]
+@[simp] theorem Term.subst_neq {t₁ t₂ : Term 𝓛} :
+  (t₁ ≉ t₂)[σ]ₚ = t₁[σ]ₜ ≉ t₂[σ]ₜ := by simp [Term.neq]
+@[simp] theorem Term.shift_eq {t₁ t₂ : Term 𝓛} :
+  ↑ₚ(t₁ ≈ t₂) = ↑ₜt₁ ≈ ↑ₜ t₂ := Term.subst_eq
 
-@[simp] theorem BTerm.unbounded_eq {t₁ t₂ : BTerm 𝓛 m} : (t₁ ≈ᵇ t₂ : Formula 𝓛) = t₁ ≈ t₂ := by simp [BTerm.eq, Term.eq]
-@[simp] theorem BTerm.unbounded_neq {t₁ t₂ : BTerm 𝓛 m} : (t₁ ≉ᵇ t₂ : Formula 𝓛) = t₁ ≉ t₂ := by simp [BTerm.neq, Term.neq]
-
+@[simp] theorem BTerm.ub_eq {t₁ t₂ : BTerm 𝓛 m} :
+  (t₁ ≈ᵇ t₂).ub = t₁.ub ≈ t₂.ub := by simp [BTerm.eq, Term.eq]
+@[simp] theorem BTerm.ub_neq {t₁ t₂ : BTerm 𝓛 m} :
+  (t₁ ≉ᵇ t₂).ub = t₁.ub ≉ t₂.ub := by simp [BTerm.neq, Term.neq]
 @[simp] theorem BTerm.subst_eq {t₁ t₂ : BTerm 𝓛 m} {σ : BSubst 𝓛 m k} : (t₁ ≈ᵇ t₂)[σ]ₚᵇ = t₁[σ]ₜᵇ ≈ᵇ t₂[σ]ₜᵇ := by simp [BTerm.eq]
 @[simp] theorem BTerm.subst_neq {t₁ t₂ : BTerm 𝓛 m} {σ : BSubst 𝓛 m k} : (t₁ ≉ᵇ t₂)[σ]ₚᵇ = t₁[σ]ₜᵇ ≉ᵇ t₂[σ]ₜᵇ := by simp [BTerm.neq]
 
@@ -62,11 +66,8 @@ namespace Proof
 
 variable {𝓣 : Theory 𝓛} [EqTheory 𝓣]
 
-theorem refl {t : Term 𝓛} : 𝓣 ⊢ t ≈ t := by
-  have h : 𝓣 ⊢ (∀ᵇ (#ᵇ0 ≈ᵇ #ᵇ0) : Sentence 𝓛) := by
-    apply Theory.axioms
-    apply EqTheory.eqAxioms
-    apply EQ.e1
+theorem refl {t : Term 𝓛} : 𝓣 ⊢ᵀ t ≈ t := by
+  have h := Theory.axioms $ EqTheory.eqAxioms (𝓣 := 𝓣) EQ.e1
   simp at h
   apply Proof.mp (Proof.forall_elim (t := t)) at h
   simp [Subst.single] at h
@@ -74,7 +75,7 @@ theorem refl {t : Term 𝓛} : 𝓣 ⊢ t ≈ t := by
 
 macro "prefl" : tactic => `(tactic| exact weaken (by pweaken_ctx) refl)
 
-theorem refl_terms {ts : Terms 𝓛 n} : 𝓣 ⊢ ts ≋ ts :=
+theorem refl_terms {ts : Terms 𝓛 n} : 𝓣 ⊢ᵀ ts ≋ ts :=
   match ts with
   | []ₜ => Proof.true_intro
   | t ∷ₜ ts => by
@@ -83,22 +84,18 @@ theorem refl_terms {ts : Terms 𝓛 n} : 𝓣 ⊢ ts ≋ ts :=
     · apply refl_terms
 
 theorem subst {t₁ t₂ : Term 𝓛} {p : Formula 𝓛} :
-  𝓣 ⊢ t₁ ≈ t₂ ⇒ p[↦ₛ t₁]ₚ ⇒ p[↦ₛ t₂]ₚ := by
+  𝓣 ⊢ᵀ t₁ ≈ t₂ ⇒ p[↦ₛ t₁]ₚ ⇒ p[↦ₛ t₂]ₚ := by
   let m := max p.bound (max t₁.bound t₂.bound)
-  let t₁' := t₁.bounded (m := m) (by simp [m])
-  let t₂' := t₂.bounded (m := m) (by simp [m])
-  let p' := p.bounded (m := m + 1) (by simp [m, Nat.le_succ_of_le])
-  have h : 𝓣 ⊢ ∀* ((t₁' ≈ᵇ t₂') ⇒ p'[↦ᵇ t₁']ₚᵇ ⇒ p'[↦ᵇ t₂']ₚᵇ) := by
-    apply Theory.axioms
-    apply EqTheory.eqAxioms
-    apply EQ.e2
+  let t₁' := t₁.bd (m := m) (by simp [m])
+  let t₂' := t₂.bd (m := m) (by simp [m])
+  let p' := p.bd (m := m + 1) (by simp [m, Nat.le_succ_of_le])
+  have h := Theory.axioms $ EqTheory.eqAxioms (𝓣 := 𝓣) $ @EQ.e2 _ _ _ t₁' t₂' p'
   apply Proof.mp Sentence.foralls_elim_self at h
-  simp [Term.bounded_unbounded, Formula.bounded_subst_single_unbounded,
-    t₁', t₂', p'] at h
+  simp [Term.bd_ub, Formula.bd_subst_single_ub, t₁', t₂', p'] at h
   exact h
 
 theorem symm {t₁ t₂ : Term 𝓛} :
-  𝓣 ⊢ t₁ ≈ t₂ ⇒ t₂ ≈ t₁ := by
+  𝓣 ⊢ᵀ t₁ ≈ t₂ ⇒ t₂ ≈ t₁ := by
   pintro
   have h := subst (𝓣 := 𝓣) (t₁ := t₁) (t₂ := t₂) (p := #0 ≈ ↑ₜt₁)
   simp [Term.shift_subst_single] at h
@@ -109,7 +106,7 @@ theorem symm {t₁ t₂ : Term 𝓛} :
 macro "psymm" : tactic => `(tactic| (apply mp (weaken (by pweaken_ctx) symm)))
 
 theorem symm_terms {ts₁ ts₂ : Terms 𝓛 n} :
-  𝓣 ⊢ ts₁ ≋ ts₂ ⇒ ts₂ ≋ ts₁ :=
+  𝓣 ⊢ᵀ ts₁ ≋ ts₂ ⇒ ts₂ ≋ ts₁ :=
   match ts₁, ts₂ with
   | []ₜ, []ₜ => Proof.identity
   | t₁ ∷ₜ ts₁, t₂ ∷ₜ ts₂ => by
@@ -123,7 +120,7 @@ theorem symm_terms {ts₁ ts₂ : Terms 𝓛 n} :
       passumption
 
 theorem trans {t₁ t₂ t₃ : Term 𝓛} :
-  𝓣 ⊢ t₁ ≈ t₂ ⇒ t₂ ≈ t₃ ⇒ t₁ ≈ t₃ := by
+  𝓣 ⊢ᵀ t₁ ≈ t₂ ⇒ t₂ ≈ t₃ ⇒ t₁ ≈ t₃ := by
   pintro
   have h := subst (𝓣 := 𝓣) (t₁ := t₂) (t₂ := t₁) (p := #0 ≈ ↑ₜt₃)
   simp [Term.shift_subst_single] at h
@@ -139,14 +136,14 @@ macro_rules
 | `(tactic| ptrans $t) => `(tactic| (apply mp2 (weaken (by pweaken_ctx) (trans (t₂ := $t)))))
 
 theorem subst_iff {t₁ t₂ : Term 𝓛} {p : Formula 𝓛} :
-  𝓣 ⊢ t₁ ≈ t₂ ⇒ (p[↦ₛ t₁]ₚ ⇔ p[↦ₛ t₂]ₚ) := by
+  𝓣 ⊢ᵀ t₁ ≈ t₂ ⇒ (p[↦ₛ t₁]ₚ ⇔ p[↦ₛ t₂]ₚ) := by
   pintro
   apply Proof.mp2 Proof.iff_intro <;> apply Proof.mp (Proof.weaken_add subst)
   · passumption
   · psymm; passumption
 
 theorem subst_term {t t₁ t₂ : Term 𝓛} :
-  𝓣 ⊢ t₁ ≈ t₂ ⇒ t[↦ₛ t₁]ₜ ≈ t[↦ₛ t₂]ₜ := by
+  𝓣 ⊢ᵀ t₁ ≈ t₂ ⇒ t[↦ₛ t₁]ₜ ≈ t[↦ₛ t₂]ₜ := by
   pintro
   have h := subst (𝓣 := 𝓣) (t₁ := t₁) (t₂ := t₂) (p := ↑ₜ(t[↦ₛ t₁]ₜ) ≈ t)
   simp [Term.shift_subst_single] at h
@@ -163,7 +160,7 @@ lemma cast_func {f : 𝓛.𝓕 n} {ts₁ : Terms 𝓛 n} {ts₂ : Terms 𝓛 m} 
 
 lemma congr_func_aux
   {f : 𝓛.𝓕 (n + m)} {ts₁ ts₂ : Terms 𝓛 n} {ts : Terms 𝓛 m} :
-  𝓣 ⊢ ts₁ ≋ ts₂ ⇒ f ⬝ₜ (ts ++ ts₁) ≈ f ⬝ₜ (ts ++ ts₂) :=
+  𝓣 ⊢ᵀ ts₁ ≋ ts₂ ⇒ f ⬝ₜ (ts ++ ts₁) ≈ f ⬝ₜ (ts ++ ts₂) :=
   match n, ts₁, ts₂ with
   | 0, []ₜ, []ₜ => by pintro; prefl
   | n + 1, t₁ ∷ₜ ts₁, t₂ ∷ₜ ts₂ => by
@@ -182,7 +179,7 @@ lemma congr_func_aux
       passumption
 
 theorem congr_func {f : 𝓛.𝓕 n} {ts₁ ts₂ : Terms 𝓛 n} :
-  𝓣 ⊢ ts₁ ≋ ts₂ ⇒ f ⬝ₜ ts₁ ≈ f ⬝ₜ ts₂ :=
+  𝓣 ⊢ᵀ ts₁ ≋ ts₂ ⇒ f ⬝ₜ ts₁ ≈ f ⬝ₜ ts₂ :=
   congr_func_aux (ts := []ₜ)
 
 lemma cast_atom {p : 𝓛.𝓟 n} {ts₁ : Terms 𝓛 n} {ts₂ : Terms 𝓛 m} (h : n = m) :
@@ -194,7 +191,7 @@ lemma cast_atom {p : 𝓛.𝓟 n} {ts₁ : Terms 𝓛 n} {ts₂ : Terms 𝓛 m} 
 
 lemma congr_atom_aux
   {p : 𝓛.𝓟 (n + m)} {ts₁ ts₂ : Terms 𝓛 n} {ts : Terms 𝓛 m} :
-  𝓣 ⊢ ts₁ ≋ ts₂ ⇒ p ⬝ₚ (ts ++ ts₁) ⇒ p ⬝ₚ (ts ++ ts₂) :=
+  𝓣 ⊢ᵀ ts₁ ≋ ts₂ ⇒ p ⬝ₚ (ts ++ ts₁) ⇒ p ⬝ₚ (ts ++ ts₂) :=
   match n, ts₁, ts₂ with
   | 0, []ₜ, []ₜ => by pintro; exact Proof.identity
   | n + 1, t₁ ∷ₜ ts₁, t₂ ∷ₜ ts₂ => by
@@ -213,11 +210,11 @@ lemma congr_atom_aux
       passumption
 
 theorem congr_atom {p : 𝓛.𝓟 n} {ts₁ ts₂ : Terms 𝓛 n} :
-  𝓣 ⊢ ts₁ ≋ ts₂ ⇒ p ⬝ₚ ts₁ ⇒ p ⬝ₚ ts₂ :=
+  𝓣 ⊢ᵀ ts₁ ≋ ts₂ ⇒ p ⬝ₚ ts₁ ⇒ p ⬝ₚ ts₂ :=
   congr_atom_aux (ts := []ₜ)
 
 theorem congr_atom_iff {p : 𝓛.𝓟 n} {ts₁ ts₂ : Terms 𝓛 n} :
-  𝓣 ⊢ ts₁ ≋ ts₂ ⇒ (p ⬝ₚ ts₁ ⇔ p ⬝ₚ ts₂) := by
+  𝓣 ⊢ᵀ ts₁ ≋ ts₂ ⇒ (p ⬝ₚ ts₁ ⇔ p ⬝ₚ ts₂) := by
   pintro
   apply Proof.mp2 Proof.iff_intro <;> apply Proof.mp (Proof.weaken_add congr_atom)
   · passumption
